# 12.4

When $T(N)= 2T\left(\frac{N}{2}\right) + O(N^2)$,
$
\begin{align*}
T(N) &= 2T\left(\frac{N}{2}\right) + O(N^2) \\
     &= 2 *\left(2T\left(\frac{N}{4}\right) + O\left(\frac{N^2}{4}\right)\right) + O(N^2) \\
     &= 4T\left(\frac{N}{4}\right) + 2O\left(\frac{N^2}{4}\right)+ O(N^2) \\
     &= 2^m*T\left(\frac{N}{2^m}\right) +\sum_{k=1}^{m} 2k*O\left(\frac{N^2}{2^{2k}}\right)+ O(N^2)\\
     &= O(N^2),
\end{align*}
$
where $m$ is natural number.

When $T(N)= 2T\left(\frac{N}{2}\right) + O(N\log(N))$,
$
\begin{align*}
T(N) &= 2T\left(\frac{N}{2}\right) + O(N\log(N)) \\
     &= 2 *\left(2T\left(\frac{N}{4}\right) + O\left(\frac{N}{2}\log\left(\frac{N}{2}\right)\right)\right) + O(N\log(N)) \\
     &= 4T\left(\frac{N}{4}\right) + 2O\left(\frac{N}{2}\log\left(\frac{N}{2}\right)\right) + O(N\log(N)) \\
     &= 2^m*T\left(\frac{N}{2^m}\right) +\sum_{k=1}^{m} 2k*O\left(\frac{N}{2^k}\log\left(\frac{N}{2^k}\right)\right)+ O(N\log(N))\\
     &= O(N\log(N)),
\end{align*}
$
where $m$ is natural number.